kvt_map introduced to store read version's writer tid, and necessary changes

txn-data-consistency/CCv_Eiger_Port_modified.thy
@@ -39,7 +39,7 @@ definition DS_init :: "'v datastore" where
   "DS_init \<equiv> (\<lambda>k. DS_vl_init)"
 
 \<comment> \<open>Client State\<close>
-datatype 'v state_txn = Idle | RtxnInProg "key set" "key \<rightharpoonup> 'v" | WtxnPrep "key \<rightharpoonup> 'v" |
+datatype 'v state_txn = Idle | RtxnInProg "key set" "key \<rightharpoonup> ('v \<times> txid)" | WtxnPrep "key \<rightharpoonup> 'v" |
   WtxnCommit tstmp tstmp "key \<rightharpoonup> 'v"
 type_synonym view_txid = "key \<Rightarrow> txid set"
 
@@ -339,7 +339,7 @@ lemma commit_in_vl_ver_in_set:
 subsubsection \<open>Simulation function\<close>
 
 definition pending_rtxn :: "'v state \<Rightarrow> txid0 \<Rightarrow> bool" where
-  "pending_rtxn s t \<equiv> \<exists>keys kv_map. txn_state (cls s (get_cl_txn t)) = RtxnInProg keys kv_map \<and>
+  "pending_rtxn s t \<equiv> \<exists>keys kvt_map. txn_state (cls s (get_cl_txn t)) = RtxnInProg keys kvt_map \<and>
     txn_sn (cls s (get_cl_txn t)) = get_sn_txn t"
 
 definition pending_wtxn :: "'v state \<Rightarrow> txid \<Rightarrow> bool" where
@@ -401,8 +401,8 @@ lemmas get_state_defs = epv_to_ver_def get_ver_committed_rd_def get_vl_pre_commi
 \<comment> \<open>Lemmas about simulation functions\<close>
 
 lemma pending_rtxn_inv:
-  assumes "\<forall>keys kv_map. txn_state (cls s cl) \<noteq> RtxnInProg keys kv_map"
-    and "\<forall>keys kv_map. txn_state (cls s' cl) \<noteq> RtxnInProg keys kv_map"
+  assumes "\<forall>keys kvt_map. txn_state (cls s cl) \<noteq> RtxnInProg keys kvt_map"
+    and "\<forall>keys kvt_map. txn_state (cls s' cl) \<noteq> RtxnInProg keys kvt_map"
     and "\<forall>cl'. cl' \<noteq> cl \<longrightarrow> cls s' cl' = cls s cl'"
   shows "pending_rtxn s' t = pending_rtxn s t"
   using assms
@@ -410,7 +410,7 @@ lemma pending_rtxn_inv:
 
 lemma pending_rtxn_added:
   assumes "txn_state (cls s cl) = Idle"
-    and "txn_state (cls s' cl) = RtxnInProg keys kv_map"
+    and "txn_state (cls s' cl) = RtxnInProg keys kvt_map"
     and "txn_sn (cls s' cl) = txn_sn (cls s cl)"
     and "\<forall>cl'. cl' \<noteq> cl \<longrightarrow> cls s' cl' = cls s cl'"
   shows "Collect (pending_rtxn s') = insert (get_txn_cl s cl) (Collect (pending_rtxn s))"
@@ -419,7 +419,7 @@ lemma pending_rtxn_added:
      apply (metis get_cl_txn.elims get_sn_txn.simps) by metis+
 
 lemma pending_rtxn_removed:
-  assumes "txn_state (cls s cl) = RtxnInProg keys kv_map"
+  assumes "txn_state (cls s cl) = RtxnInProg keys kvt_map"
     and "txn_state (cls s' cl) = Idle"
     and "txn_sn (cls s' cl) = txn_sn (cls s cl)"
     and "\<forall>cl'. cl' \<noteq> cl \<longrightarrow> cls s' cl' = cls s cl'"
@@ -505,7 +505,7 @@ lemma get_vl_pre_committed_readersets:
 subsubsection \<open>Events\<close>
 
 datatype 'v ev =
-  RInvoke cl_id "key set" | Read cl_id key 'v | RDone cl_id "key \<rightharpoonup> 'v" sqn view |
+  RInvoke cl_id "key set" | Read cl_id key 'v txid | RDone cl_id "key \<rightharpoonup> ('v \<times> txid)" sqn view |
   WInvoke cl_id "key \<rightharpoonup> 'v" | WCommit cl_id "key \<rightharpoonup> 'v" tstmp sqn view | WDone cl_id |
   RegR svr_id txid0 'v txid tstmp | PrepW svr_id txid0 'v tstmp | CommitW svr_id txid0 | Skip2
 
@@ -543,16 +543,16 @@ definition read_invoke :: "cl_id \<Rightarrow> key set \<Rightarrow> 'v state \<
     svrs_cls_cl'_unchanged cl s s' \<and>
     global_time s' = Suc (global_time s)"
 
-fun find_and_read_val :: "'v epv_list \<Rightarrow> txid0 \<rightharpoonup> 'v" where
+fun find_and_read_val :: "'v epv_list \<Rightarrow> txid0 \<rightharpoonup> ('v \<times> txid)" where
   "find_and_read_val [] t = None" |
   "find_and_read_val (ver # vl) t =
-    (if t \<in> v_readerset ver then Some (v_value ver) else find_and_read_val vl t)"
+    (if t \<in> v_readerset ver then Some (v_value ver, v_writer ver) else find_and_read_val vl t)"
 
-definition read :: "cl_id \<Rightarrow> key \<Rightarrow> 'v \<Rightarrow> 'v state \<Rightarrow> 'v state \<Rightarrow> bool" where
-  "read cl k v s s' \<equiv> (\<exists>keys vals.
+definition read :: "cl_id \<Rightarrow> key \<Rightarrow> 'v \<Rightarrow> txid \<Rightarrow> 'v state \<Rightarrow> 'v state \<Rightarrow> bool" where
+  "read cl k v t s s' \<equiv> (\<exists>keys vals.
     txn_state (cls s cl) = RtxnInProg keys vals \<and> k \<in> keys \<and> vals k = None \<and>
-    txn_state (cls s' cl) = RtxnInProg keys (vals (k \<mapsto> v))) \<and>
-    Some v = find_and_read_val (DS (svrs s k)) (get_txn_cl s cl) \<and>
+    txn_state (cls s' cl) = RtxnInProg keys (vals (k \<mapsto> (v, t)))) \<and>
+    Some (v, t) = find_and_read_val (DS (svrs s k)) (get_txn_cl s cl) \<and>
     txn_sn (cls s' cl) = txn_sn (cls s cl) \<and>
     gst (cls s' cl) = gst (cls s cl) \<and>
     lst_map (cls s' cl) k = lst (svrs s k) \<and>
@@ -562,18 +562,20 @@ definition read :: "cl_id \<Rightarrow> key \<Rightarrow> 'v \<Rightarrow> 'v st
     svrs_cls_cl'_unchanged cl s s' \<and>
     global_time s' = Suc (global_time s)"
 
-definition read_done :: "cl_id \<Rightarrow> (key \<rightharpoonup> 'v) \<Rightarrow> sqn \<Rightarrow> view \<Rightarrow> 'v state \<Rightarrow> 'v state \<Rightarrow> bool" where
-  "read_done cl kv_map sn u'' s s' \<equiv>
+definition read_done :: "cl_id \<Rightarrow> (key \<rightharpoonup> ('v \<times> txid)) \<Rightarrow> sqn \<Rightarrow> view \<Rightarrow> 'v state \<Rightarrow> 'v state \<Rightarrow> bool" where
+  "read_done cl kvt_map sn u'' s s' \<equiv>
     sn = txn_sn (cls s cl) \<and>
-    u'' = views_of_s s' cl \<and>
-    txn_state (cls s cl) = RtxnInProg (dom kv_map) kv_map \<and>
+    u'' = view_txid_vid s (\<lambda>k. case kvt_map k of
+      Some (v, t) \<Rightarrow> insert t (cl_view (cls s cl) k) |
+      None \<Rightarrow> cl_view (cls s cl) k) \<and>
+    txn_state (cls s cl) = RtxnInProg (dom kvt_map) kvt_map \<and>
     txn_state (cls s' cl) = Idle \<and>
     txn_sn (cls s' cl) = Suc (txn_sn (cls s cl)) \<and>
     gst (cls s' cl) = gst (cls s cl) \<and>
     lst_map (cls s' cl) = lst_map (cls s cl) \<and>
-    (\<forall>k \<in> dom kv_map. cl_view (cls s' cl) k =
-      insert (ver_writer (read_at (DS (svrs s k)) (gst (cls s cl)) cl)) (cl_view (cls s cl) k)) \<and>
-    (\<forall>k. k \<notin> dom kv_map \<longrightarrow> cl_view (cls s' cl) k = cl_view (cls s cl) k) \<and>
+    cl_view (cls s' cl) = (\<lambda>k. case kvt_map k of
+      Some (v, t) \<Rightarrow> insert t (cl_view (cls s cl) k) |
+      None \<Rightarrow> cl_view (cls s cl) k) \<and>
     cl_clock (cls s' cl) = Suc (cl_clock (cls s cl)) \<and>
     svrs_cls_cl'_unchanged cl s s' \<and>
     global_time s' = Suc (global_time s)"
@@ -592,9 +594,9 @@ definition write_invoke :: "cl_id \<Rightarrow> (key \<rightharpoonup> 'v) \<Rig
     global_time s' = Suc (global_time s)"
 
 definition write_commit :: "cl_id \<Rightarrow> (key \<rightharpoonup> 'v) \<Rightarrow> tstmp \<Rightarrow> sqn \<Rightarrow> view \<Rightarrow> 'v state \<Rightarrow> 'v state \<Rightarrow> bool" where
-  "write_commit cl kv_map commit_t sn u s s' \<equiv>
+  "write_commit cl kv_map commit_t sn u'' s s' \<equiv>
     sn = txn_sn (cls s cl) \<and>
-    u = views_of_s s cl \<and>
+    u'' = views_of_s s cl \<and>
     txn_state (cls s cl) = WtxnPrep kv_map \<and>
     (\<forall>k \<in> dom kv_map.
       (\<exists>prep_t. wtxn_state (svrs s k) (get_txn_cl s cl) = Prep prep_t) \<and>
@@ -629,9 +631,9 @@ definition write_done :: "cl_id \<Rightarrow> 'v state \<Rightarrow> 'v state \<
 definition register_read :: "svr_id \<Rightarrow> txid0 \<Rightarrow> 'v \<Rightarrow> txid \<Rightarrow> tstmp \<Rightarrow> 'v state \<Rightarrow> 'v state \<Rightarrow> bool" where
   "register_read svr t v t' gst_ts s s' \<equiv>
     tid_match s t \<and>
-    (\<exists>keys vals.
-      txn_state (cls s (get_cl_txn t)) = RtxnInProg keys vals \<and> svr \<in> keys \<and> vals svr = None) \<and>
-    \<lparr>ver_val = v, ver_writer = t' \<rparr> = read_at (DS (svrs s svr)) gst_ts (get_cl_txn t) \<and>
+    (\<exists>keys kvt_map.
+      txn_state (cls s (get_cl_txn t)) = RtxnInProg keys kvt_map \<and> svr \<in> keys \<and> kvt_map svr = None) \<and>
+    \<lparr>ver_val = v, ver_writer = t'\<rparr> = read_at (DS (svrs s svr)) gst_ts (get_cl_txn t) \<and>
     gst_ts = gst (cls s (get_cl_txn t)) \<and>
     wtxn_state (svrs s' svr) = wtxn_state (svrs s svr) \<and>
     clock (svrs s' svr) = Suc (clock (svrs s svr)) \<and>
@@ -703,15 +705,15 @@ definition state_init :: "'v state" where
   \<rparr>"
 
 fun state_trans :: "'v state \<Rightarrow> 'v ev \<Rightarrow> 'v state \<Rightarrow> bool" where
-  "state_trans s (RInvoke cl keys)        s' \<longleftrightarrow> read_invoke cl keys s s'" |
-  "state_trans s (Read cl k v)            s' \<longleftrightarrow> read cl k v s s'" |
-  "state_trans s (RDone cl kv_map sn u)   s' \<longleftrightarrow> read_done cl kv_map sn u s s'" |
-  "state_trans s (WInvoke cl kv_map)      s' \<longleftrightarrow> write_invoke cl kv_map s s'" |
-  "state_trans s (WCommit cl kv_map cts sn u)  s' \<longleftrightarrow> write_commit cl kv_map cts sn u s s'" |
-  "state_trans s (WDone cl)               s' \<longleftrightarrow> write_done cl s s'" |
-  "state_trans s (RegR svr t v i gts)     s' \<longleftrightarrow> register_read svr t v i gts s s'" |
-  "state_trans s (PrepW svr t v gts)      s' \<longleftrightarrow> prepare_write svr t v gts s s'" |
-  "state_trans s (CommitW svr t)          s' \<longleftrightarrow> commit_write svr t s s'" |
+  "state_trans s (RInvoke cl keys)          s' \<longleftrightarrow> read_invoke cl keys s s'" |
+  "state_trans s (Read cl k v t)            s' \<longleftrightarrow> read cl k v t s s'" |
+  "state_trans s (RDone cl kvt_map sn u'')  s' \<longleftrightarrow> read_done cl kvt_map sn u'' s s'" |
+  "state_trans s (WInvoke cl kv_map)        s' \<longleftrightarrow> write_invoke cl kv_map s s'" |
+  "state_trans s (WCommit cl kv_map cts sn u'')  s' \<longleftrightarrow> write_commit cl kv_map cts sn u'' s s'" |
+  "state_trans s (WDone cl)                 s' \<longleftrightarrow> write_done cl s s'" |
+  "state_trans s (RegR svr t v i gts)       s' \<longleftrightarrow> register_read svr t v i gts s s'" |
+  "state_trans s (PrepW svr t v gts)        s' \<longleftrightarrow> prepare_write svr t v gts s s'" |
+  "state_trans s (CommitW svr t)            s' \<longleftrightarrow> commit_write svr t s s'" |
   "state_trans s Skip2 s' \<longleftrightarrow> s' = s"
 
 definition tps :: "('v ev, 'v state) ES" where
@@ -727,9 +729,13 @@ lemmas tps_defs = tps_def state_init_def
 
 lemma tps_trans [simp]: "trans tps = state_trans" by (simp add: tps_def)
 
+term image
+definition o_fst :: "('a \<Rightarrow> ('b \<times> 'c) option) \<Rightarrow> 'a \<Rightarrow> 'b option" where
+  "o_fst m \<equiv> (\<lambda>a. case m a of None \<Rightarrow> None | Some (b, c) \<Rightarrow> Some b)"
+
 \<comment> \<open>Mediator function\<close>
 fun med :: "'v ev \<Rightarrow> 'v label" where
-  "med (RDone cl kv_map sn u'') = ET cl sn u'' (\<lambda>k op. case op of R \<Rightarrow> kv_map k | W \<Rightarrow> None)" |
+  "med (RDone cl kvt_map sn u'') = ET cl sn u'' (\<lambda>k op. case op of R \<Rightarrow> o_fst kvt_map k | W \<Rightarrow> None)" |
   "med (WCommit cl kv_map _ sn u'') = ET cl sn u'' (\<lambda>k op. case op of R \<Rightarrow> None | W \<Rightarrow> kv_map k)" |
   "med _ = ETSkip"
 
@@ -802,7 +808,7 @@ proof (induction e)
   then show ?case apply (auto simp add: read_invoke_def cl_unchanged_defs)
     by (metis Suc_n_not_le_n nat_le_linear)
 next
-  case (Read x1 x2 x3)
+  case (Read x1 x2 x3 x4)
   then show ?case apply (auto simp add: read_def cl_unchanged_defs)
     by (metis Suc_n_not_le_n max.coboundedI1 nat_le_linear)
 next
@@ -1165,7 +1171,7 @@ next
     then show ?case apply (auto simp add: CommitGltsNotZero_def tps_trans_defs cl_unchanged_defs)
       by (metis state_txn.distinct(9))
   next
-    case (Read x1 x2 x3)
+    case (Read x1 x2 x3 x4)
     then show ?case apply (auto simp add: CommitGltsNotZero_def tps_trans_defs cl_unchanged_defs)
       by (metis state_txn.distinct(9))
   next
@@ -1315,7 +1321,7 @@ next
         apply (smt (verit) state_txn.distinct(5) txid.simps(5) txid0.case)
         by (smt (verit, ccfv_threshold) txid.simps(5) txid0.case).
   next
-    case (Read x1 x2 x3)
+    case (Read x1 x2 x3 x4)
     then show ?case apply (auto simp add: ReadyToCommitVer_def tps_trans_defs cl_unchanged_defs
           get_state_defs pending_wtxn_def)
       by (smt (z3) state_txn.distinct(7) state_txn.distinct(9) txid.simps(5) txid0.case)+
@@ -1392,7 +1398,7 @@ next
     then show ?case
       by (auto simp add: tps_trans_defs cl_unchanged_defs tid_match_def FutureTIDInv_def, metis)
   next
-    case (Read x21 x22 x23)
+    case (Read x21 x22 x23 x24)
     then show ?case
       by (auto simp add: tps_trans_defs cl_unchanged_defs tid_match_def FutureTIDInv_def, metis)
   next
@@ -1451,13 +1457,13 @@ next
     then show ?case apply (simp add: IdleReadInv_def tps_trans_defs cl_unchanged_defs)
       by metis
   next
-    case (Read x1 x2 x3)
+    case (Read x1 x2 x3 x4)
     then show ?case apply (simp add: IdleReadInv_def tps_trans_defs cl_unchanged_defs)
       by metis
   next
     case (RDone x1 x2 x3 x4)
     then show ?case apply (simp add: IdleReadInv_def tps_trans_defs cl_unchanged_defs)
-      by (metis FutureTIDInv_def lessI reach_tidfuturekm)
+      by (metis (opaque_lifting) FutureTIDInv_def lessI reach_tidfuturekm)
   next
     case (WInvoke x1 x2)
     then show ?case apply (simp add: IdleReadInv_def tps_trans_defs cl_unchanged_defs)
@@ -1506,13 +1512,13 @@ next
     then show ?case apply (simp add: WriteTxnIdleSvr_def tps_trans_defs cl_unchanged_defs)
       by (metis state_txn.distinct(7) state_txn.distinct(9))
   next
-    case (Read x1 x2 x3)
+    case (Read x1 x2 x3 x4)
     then show ?case apply (simp add: WriteTxnIdleSvr_def tps_trans_defs cl_unchanged_defs)
       by (metis state_txn.distinct(7) state_txn.distinct(9))
   next
     case (RDone x1 x2 x3 x4)
     then show ?case apply (simp add: WriteTxnIdleSvr_def tps_trans_defs cl_unchanged_defs)
-      by (metis state_txn.distinct(3) state_txn.distinct(5))
+      by (metis (lifting) state_txn.distinct(3) state_txn.distinct(5))
   next
     case (WInvoke x1 x2)
     then show ?case apply (auto simp add: WriteTxnIdleSvr_def tps_trans_defs cl_unchanged_defs)
@@ -1630,13 +1636,13 @@ next
     then show ?case apply (simp add: PrepInv_def tps_trans_defs cl_unchanged_defs)
       by (metis state_txn.distinct(7))
   next
-    case (Read x1 x2 x3)
+    case (Read x1 x2 x3 x4)
     then show ?case apply (simp add: PrepInv_def tps_trans_defs cl_unchanged_defs)
       by (metis state_txn.distinct(7))
   next
     case (RDone x1 x2 x3 x4)
     then show ?case apply (simp add: PrepInv_def tps_trans_defs cl_unchanged_defs)
-      by (metis state_txn.distinct(3))
+      by (metis (lifting) state_txn.distinct(3))
   next
     case (WInvoke x1 x2)
     then show ?case apply (simp add: PrepInv_def tps_trans_defs cl_unchanged_defs)
@@ -1684,13 +1690,13 @@ next
     then show ?case apply (simp add: CommitInv_def tps_trans_defs cl_unchanged_defs)
       by (metis state_txn.distinct(9))
   next
-    case (Read x1 x2 x3)
+    case (Read x1 x2 x3 x4)
     then show ?case apply (simp add: CommitInv_def tps_trans_defs cl_unchanged_defs)
       by (metis state_txn.distinct(9))
   next
     case (RDone x1 x2 x3 x4)
     then show ?case apply (simp add: CommitInv_def tps_trans_defs cl_unchanged_defs)
-      by (metis state_txn.distinct(5))
+      by (metis (lifting) state_txn.distinct(5))
   next
     case (WInvoke x1 x2)
     then show ?case apply (simp add: CommitInv_def tps_trans_defs cl_unchanged_defs)
@@ -1736,7 +1742,7 @@ next
     case (RInvoke x1 x2)
     then show ?case by (simp add: FutureTidRdDS_def tps_trans_defs cl_unchanged_defs, metis)
   next
-    case (Read x1 x2 x3)
+    case (Read x1 x2 x3 x4)
     then show ?case by (simp add: FutureTidRdDS_def tps_trans_defs cl_unchanged_defs, metis)
   next
     case (RDone x1 x2 x3 x4)
@@ -1834,7 +1840,7 @@ next
     case (RInvoke x1 x2)
     then show ?case by (simp add: VerWrLCurrT_def tps_trans_defs cl_unchanged_defs, metis)
   next
-    case (Read x1 x2 x3)
+    case (Read x1 x2 x3 x4)
     then show ?case by (simp add: VerWrLCurrT_def tps_trans_defs cl_unchanged_defs, metis)
   next
     case (RDone x1 x2 x3 x4)
@@ -1891,12 +1897,12 @@ next
     case (RInvoke x1 x2)
     then show ?case by (simp add: VerWrLCurrT2_def tps_trans_defs cl_unchanged_defs, metis)
   next
-    case (Read x1 x2 x3)
+    case (Read x1 x2 x3 x4)
     then show ?case by (simp add: VerWrLCurrT2_def tps_trans_defs cl_unchanged_defs, metis)
   next
     case (RDone x1 x2 x3 x4)
     then show ?case apply (simp add: VerWrLCurrT2_def tps_trans_defs cl_unchanged_defs)
-      by (metis less_SucI)
+      by (metis (lifting) less_SucI)
   next
     case (WInvoke x1 x2)
     then show ?case by (simp add: VerWrLCurrT2_def tps_trans_defs cl_unchanged_defs, metis)
@@ -1943,12 +1949,12 @@ next
     case (RInvoke x1 x2)
     then show ?case by (simp add: VerWrLCurrT3_def tps_trans_defs cl_unchanged_defs, metis)
   next
-    case (Read x1 x2 x3)
+    case (Read x1 x2 x3 x4)
     then show ?case by (simp add: VerWrLCurrT3_def tps_trans_defs cl_unchanged_defs, metis)
   next
     case (RDone x1 x2 x3 x4)
     then show ?case apply (simp add: VerWrLCurrT3_def tps_trans_defs cl_unchanged_defs)
-      by (metis VerWrLCurrT2_def insert_iff less_Suc_eq reach_ver_wr_L_currT2)
+      by (metis (no_types, lifting) VerWrLCurrT2_def insertCI less_Suc_eq reach_ver_wr_L_currT2)
   next
     case (WInvoke x1 x2)
     then show ?case by (simp add: VerWrLCurrT3_def tps_trans_defs cl_unchanged_defs, metis)
@@ -2027,12 +2033,12 @@ next
     case (RInvoke x1 x2)
     then show ?case by (simp add: PastTIDNotPending_def tps_trans_defs cl_unchanged_defs, metis)
   next
-    case (Read x1 x2 x3)
+    case (Read x1 x2 x3 x4)
     then show ?case by (simp add: PastTIDNotPending_def tps_trans_defs cl_unchanged_defs, metis)
   next
     case (RDone x1 x2 x3 x4)
     then show ?case apply (simp add: PastTIDNotPending_def tps_trans_defs cl_unchanged_defs)
-      by (metis VerWrLCurrT2_def insertCI reach_ver_wr_L_currT2)
+      by (metis (lifting) VerWrLCurrT2_def insertCI reach_ver_wr_L_currT2)
   next
     case (WInvoke x1 x2)
     then show ?case by (simp add: PastTIDNotPending_def tps_trans_defs cl_unchanged_defs, metis)
@@ -2063,7 +2069,7 @@ qed
 
 
 abbreviation not_committing_ev where
-  "not_committing_ev e \<equiv> \<forall>cl kv_map cts sn u. e \<noteq> RDone cl kv_map sn u \<and> e \<noteq> WCommit cl kv_map cts sn u"
+  "not_committing_ev e \<equiv> \<forall>cl kvt_map kv_map cts sn u. e \<noteq> RDone cl kvt_map sn u \<and> e \<noteq> WCommit cl kv_map cts sn u"
 
 
 definition FreshReadTxnInv where
@@ -2091,7 +2097,7 @@ next
   next
     case (RDone x31 x32 x33 x34)
     then show ?case apply (simp add: FreshReadTxnInv_def tps_trans_defs cl_unchanged_defs)
-      by (metis FutureTidRdDS_def lessI nth_mem reach_tidfuture_rd_ds)
+      by (metis (lifting) FutureTidRdDS_def lessI nth_mem reach_tidfuture_rd_ds)
   next
     case (WInvoke x41 x42)
     then show ?case by (simp add: FreshReadTxnInv_def tps_trans_defs cl_unchanged_defs, metis)
@@ -2117,7 +2123,7 @@ next
 qed
 
 definition FreshWriteTxnInv where
-  "FreshWriteTxnInv s cl \<longleftrightarrow> (\<forall>keys kv_map k. txn_state (cls s cl) \<in> {Idle, RtxnInProg keys kv_map} \<longrightarrow>
+  "FreshWriteTxnInv s cl \<longleftrightarrow> (\<forall>keys kvt_map k. txn_state (cls s cl) \<in> {Idle, RtxnInProg keys kvt_map} \<longrightarrow>
     Tn (get_txn_cl s cl) \<notin> v_writer ` set (DS (svrs s k)))"
 
 lemmas FreshWriteTxnInvI = FreshWriteTxnInv_def[THEN iffD2, rule_format]
@@ -2135,12 +2141,12 @@ next
     case (RInvoke x1 x2)
     then show ?case by (simp add: tps_trans_defs FreshWriteTxnInv_def cl_unchanged_defs, metis)
   next
-    case (Read x1 x2 x3)
+    case (Read x1 x2 x3 x4)
     then show ?case by (simp add: tps_trans_defs FreshWriteTxnInv_def cl_unchanged_defs, metis)
   next
     case (RDone x1 x2 x3 x4)
     then show ?case apply (simp add: tps_trans_defs FreshWriteTxnInv_def cl_unchanged_defs)
-      by (metis FutureTidWrDS_def lessI reach_tidfuture_wr_ds)
+      by (metis (lifting) FutureTidWrDS_def lessI reach_tidfuture_wr_ds)
   next
     case (WInvoke x1 x2)
     then show ?case by (simp add: tps_trans_defs FreshWriteTxnInv_def cl_unchanged_defs, metis)
@@ -2193,7 +2199,7 @@ lemma kvs_of_s_inv:
       apply (auto simp add: tps_trans_defs kvs_of_s_def cl_unchanged_defs get_vl_pre_committed_readersets)
       apply (rule ext) sorry
   next
-    case (Read x1 x2 x3)
+    case (Read x1 x2 x3 x4)
     then show ?case sorry
   next
     case (WInvoke x1 x2)
@@ -2223,7 +2229,7 @@ proof (induction e)
   then show ?case using pending_wtxn_cl_ev_inv[of s x1 s']
     by (simp add: tps_trans_defs get_vl_pre_committed_writers cl_unchanged_defs)
 next
-  case (Read x1 x2 x3)
+  case (Read x1 x2 x3 x4)
   then show ?case using pending_wtxn_cl_ev_inv[of s x1 s']
     apply (simp add: tps_trans_defs get_vl_pre_committed_writers cl_unchanged_defs)
     by (metis state_txn.distinct(7))
@@ -2340,7 +2346,7 @@ lemma prefix_subset_indices_map:
   by (metis map_extend_subset dom_indices_map prefix_update_get_indices_map)
 
 lemma read_commit_indices_map_grows:
-  assumes "read_done cl kv_map sn u s s'"
+  assumes "read_done cl kvt_map sn u s s'"
   shows "get_indices_map (kvs_of_s s k) \<subseteq>\<^sub>m get_indices_map (kvs_of_s s' k)"
   using assms
   apply (induction "kvs_of_s s k"; simp add: read_done_def dom_indices_map get_indices_map_def)
@@ -2365,7 +2371,7 @@ next
     case (RInvoke x1 x2)
     then show ?case by (simp add: OnlyPendingVer_def tps_trans_defs cl_unchanged_defs, metis)
   next
-    case (Read x1 x2 x3)
+    case (Read x1 x2 x3 x4)
     then show ?case by (simp add: OnlyPendingVer_def tps_trans_defs cl_unchanged_defs, metis)
   next
     case (RDone x1 x2 x3 x4)
@@ -2397,7 +2403,7 @@ qed
 
 definition CurrentVerPending where
   "CurrentVerPending s cl k \<longleftrightarrow>
-    (\<forall>kvm keys ver. txn_state (cls s cl) \<in> {Idle, WtxnPrep kvm, RtxnInProg keys kvm} \<and> 
+    (\<forall>kvm keys ver kvtm. txn_state (cls s cl) \<in> {Idle, WtxnPrep kvm, RtxnInProg keys kvtm} \<and> 
     find (is_txn_writer (Tn (get_txn_cl s cl))) (DS (svrs s k)) = Some ver \<longrightarrow> v_is_pending ver)"
 
 lemmas CurrentVerPendingI = CurrentVerPending_def[THEN iffD2, rule_format]
@@ -2415,13 +2421,13 @@ next
     case (RInvoke x1 x2)
     then show ?case by (simp add: CurrentVerPending_def tps_trans_defs cl_unchanged_defs, metis)
   next
-    case (Read x1 x2 x3)
+    case (Read x1 x2 x3 x4)
     then show ?case by (simp add: CurrentVerPending_def tps_trans_defs cl_unchanged_defs, metis)
   next
     case (RDone x1 x2 x3 x4)
     then show ?case apply (simp add: CurrentVerPending_def tps_trans_defs cl_unchanged_defs)
-      by (metis (mono_tags) find_Some_in_set VerWrLCurrT_def Suc_n_not_le_n is_txn_writer_def
-          reach_ver_wr_L_currT)
+      by (metis (mono_tags, opaque_lifting) FutureTidWrDS_def find_Some_in_set image_iff
+          is_txn_writer_def lessI reach_tidfuture_wr_ds)
   next
     case (WInvoke x1 x2)
     then show ?case by (simp add: CurrentVerPending_def tps_trans_defs cl_unchanged_defs, metis)
@@ -2587,13 +2593,13 @@ next
     then show ?case apply (simp add: SqnInv_nc_def tps_trans_defs cl_unchanged_defs)
       by (metis state_txn.distinct(5))
   next
-    case (Read x1 x2 x3)
+    case (Read x1 x2 x3 x4)
     then show ?case apply (simp add: SqnInv_nc_def tps_trans_defs cl_unchanged_defs)
       by (metis state_txn.distinct(9))
   next
     case (RDone x1 x2 x3 x4)
     then show ?case apply (auto simp add: SqnInv_nc_def tps_trans_defs)
-       apply (metis state_txn.distinct(9) cl_unchanged_defs)
+       apply (metis (lifting) state_txn.distinct(9) cl_unchanged_defs)
       apply (cases "cl = x1", simp)
       subgoal sorry
       by (smt (verit) other_insts_unchanged_def reach_kvs_non_emp reach_tidfuturekm reach_tidpastkm
@@ -2636,7 +2642,7 @@ next
     then show ?case apply (simp add: SqnInv_c_def tps_trans_defs cl_unchanged_defs)
       by (metis state_txn.distinct(9))
   next
-    case (Read x1 x2 x3)
+    case (Read x1 x2 x3 x4)
     then show ?case apply (simp add: SqnInv_c_def tps_trans_defs cl_unchanged_defs)
       by (metis state_txn.distinct(9))
   next
@@ -2663,7 +2669,7 @@ qed
 
 lemma t_is_fresh:
   assumes "SqnInv_c s cl" and "SqnInv_nc s cl"
-    and "txn_state (cls s cl) \<in> {WtxnPrep kv_map, RtxnInProg keys kv_map}"
+    and "txn_state (cls s cl) \<in> {WtxnPrep kv_map, RtxnInProg keys kvt_map}"
   shows "get_txn_cl s cl \<in> next_txids (kvs_of_s s) cl"
   using assms by (auto simp add: kvs_of_s_def next_txids_def)
 
@@ -2685,8 +2691,8 @@ next
   then show ?case 
   proof (induction e)
     case (RegR x1 x2 x3 x4 x5)
-    then show ?case apply (auto simp add: RO_WO_Inv_def tps_trans_defs svr_unchanged_defs txid_defs)
-     using add_to_readerset_v_writer_img[of ] apply simp sorry \<comment> \<open>Continue here!\<close>
+    then show ?case apply (auto simp add: RO_WO_Inv_def tps_trans_defs svr_unchanged_defs)
+     using add_to_readerset_v_writer_img[of ] apply (simp add: txid_defs) sorry \<comment> \<open>Continue here!\<close>
   next
     case (PrepW x1 x2 x3 x4)
     then show ?case sorry
@@ -2697,13 +2703,13 @@ next
 qed
 
 lemma "kvs_txids (kvs_of_s gs) - kvs_writers (kvs_of_s gs) = Tn ` kvs_readers (kvs_of_s gs)"
-  apply (simp add: kvs_of_s_def)
+  apply (simp add: kvs_of_s_def) sorry
 
 lemma views_of_s_satisfies_ET_CC_canCommit:
-  assumes "txn_state (cls gs cl) = RtxnInProg (dom kv_map) kv_map"
-    and "\<forall>k\<in>dom kv_map. cl_view (cls gs' cl) k = insert (ver_writer (read_at (DS (svrs gs k)) (gst (cls gs cl)) cl)) (cl_view (cls gs cl) k)"
-    and "\<forall>k. k \<notin> dom kv_map \<longrightarrow> cl_view (cls gs' cl) k = cl_view (cls gs cl) k"
-  shows "ET_CC.canCommit (kvs_of_s gs) (views_of_s gs' cl) (\<lambda>k. case_op_type (kv_map k) None)"
+  assumes "txn_state (cls gs cl) = RtxnInProg (dom kvt_map) kvt_map"
+    and "u'' = (\<lambda>k. get_indices_fun gs k ` (case kvt_map k of
+      None \<Rightarrow> cl_view (cls gs cl) k | Some (v, t) \<Rightarrow> insert t (cl_view (cls gs cl) k)))"
+  shows "ET_CC.canCommit (kvs_of_s gs) u'' (\<lambda>k. case_op_type (o_fst kv_map k) None)"
   using assms
   apply (simp add: ET_CC.canCommit_def closed_def read_only_Txs_def R_CC_def R_onK_def views_of_s_def)
   sorry
@@ -2768,7 +2774,7 @@ next
   then show "ET_CC.ET_ES: sim gs\<midarrow>med a\<rightarrow> sim gs'"
   using kvs_of_s_inv[of gs a gs'] views_of_s_inv[of gs a gs']
   proof (induction a)
-    case (RDone cl kv_map sn u)
+    case (RDone cl kvt_map sn u'')
     then show ?case using p apply simp
       apply (auto simp add: read_done_def cl_unchanged_defs sim_def)
       apply (rule exI [where x="views_of_s gs' cl"]) apply auto
@@ -2783,11 +2789,11 @@ next
           by (metis RDone.prems(1) state_trans.simps(3) tps_trans).
       subgoal apply (auto simp add: fp_property_def view_snapshot_def)
         subgoal for k y apply (simp add: last_version_def kvs_of_s_def get_state_defs)
-          apply (cases "k \<in> dom kv_map"; auto) sorry
+          apply (cases "k \<in> dom kvt_map") sorry
         done
       done
   next
-    case (WCommit cl kv_map cts sn u)
+    case (WCommit cl kv_map cts sn u'')
     then show ?case using p apply simp
       apply (auto simp add: write_commit_def cl_unchanged_defs sim_def fp_property_def)
       apply (rule exI [where x="views_of_s gs' cl"]) apply auto
